Rewrite symcc transitivity enforcement in terms of set products and unions
This isn't a functional change (as shown by the equivalence proofs with
the unoptimized compiler). It previously use `flatMap` and `++` on the
policy footprint to construct transitivity constraints, but the
footprint is a set of terms, so this is more naturally expressed in set
operations.

cedar-lean/Cedar/SymCCOpt/Enforcer.lean
@@ -27,15 +27,15 @@ open Cedar.Data Cedar.Spec Factory
 Returns the ground acyclicity and transitivity assumptions for a single `CompiledPolicy`.
 -/
 public def enforceCompiledPolicy (cp : CompiledPolicy) : Set Term :=
-  let tr := cp.footprint.elts.flatMap (λ t => cp.footprint.elts.map (transitivity t · cp.εnv.entities))
-  Set.make (cp.acyclicity.elts ++ tr)
+  let tr := cp.footprint.product cp.footprint|>.map λ (t₁, t₂) => transitivity t₁ t₂ cp.εnv.entities
+  cp.acyclicity ∪ tr
 
 /--
 Returns the ground acyclicity and transitivity assumptions for a single `CompiledPolicySet`.
 -/
 public def enforceCompiledPolicySet (cpset : CompiledPolicySet) : Set Term :=
-  let tr := cpset.footprint.elts.flatMap (λ t => cpset.footprint.elts.map (transitivity t · cpset.εnv.entities))
-  Set.make (cpset.acyclicity.elts ++ tr)
+  let tr := cpset.footprint.product cpset.footprint|>.map λ (t₁, t₂) => transitivity t₁ t₂ cpset.εnv.entities
+  cpset.acyclicity ∪ tr
 
 /--
 Returns the ground acyclicity and transitivity assumptions for a pair of `CompiledPolicy`.
@@ -43,9 +43,9 @@ Caller guarantees that `cp₁` and `cp₂` were compiled for the same `εnv`.
 -/
 public def enforcePairCompiledPolicy (cp₁ : CompiledPolicy) (cp₂ : CompiledPolicy) : Set Term :=
   assert! cp₁.εnv = cp₂.εnv
-  let footprint := cp₁.footprint ++ cp₂.footprint
-  let tr := footprint.elts.flatMap (λ t => footprint.elts.map (transitivity t · cp₁.εnv.entities))
-  Set.make (cp₁.acyclicity.elts ++ cp₂.acyclicity.elts ++ tr)
+  let footprint := cp₁.footprint ∪ cp₂.footprint
+  let tr := footprint.product footprint|>.map λ (t₁, t₂) => transitivity t₁ t₂ cp₁.εnv.entities
+  cp₁.acyclicity ∪ cp₂.acyclicity ∪ tr
 
 /--
 Returns the ground acyclicity and transitivity assumptions for a pair of `CompiledPolicySet`.
@@ -53,8 +53,8 @@ Caller guarantees that `cpset₁` and `cpset₂` were compiled for the same `εn
 -/
 public def enforcePairCompiledPolicySet (cpset₁ : CompiledPolicySet) (cpset₂ : CompiledPolicySet) : Set Term :=
   assert! cpset₁.εnv = cpset₂.εnv
-  let footprint := cpset₁.footprint ++ cpset₂.footprint
-  let tr := footprint.elts.flatMap (λ t => footprint.elts.map (transitivity t · cpset₁.εnv.entities))
-  Set.make (cpset₁.acyclicity.elts ++ cpset₂.acyclicity.elts ++ tr)
+  let footprint := cpset₁.footprint ∪ cpset₂.footprint
+  let tr := footprint.product footprint|>.map λ (t₁, t₂) => transitivity t₁ t₂ cpset₁.εnv.entities
+  cpset₁.acyclicity ∪ cpset₂.acyclicity ∪ tr
 
 namespace Cedar.SymCC
